clean

NuInstructions.thy
@@ -4,13 +4,13 @@ begin
 
 section \<open>A Set of Predefined Minimal Instructions\<close>
 
-context \<phi>min_sem begin
+context \<phi>empty_sem begin
 
 subsection \<open>Throw Exception\<close>
 
 text \<open>The opcode for throwing an exception is directly \<^term>\<open>Exception\<close>\<close>
 
-lemma (in \<phi>min) throw_\<phi>app:
+lemma (in \<phi>empty) throw_\<phi>app:
   \<open>\<^bold>p\<^bold>r\<^bold>o\<^bold>c Exception \<lbrace> X \<longmapsto> (\<lambda>_::unreachable sem_value. 0) \<^bold>t\<^bold>h\<^bold>r\<^bold>o\<^bold>w\<^bold>s X \<rbrace>\<close>
   unfolding \<phi>Procedure_def by blast
 
@@ -20,7 +20,7 @@ definition op_try :: "('ret,'RES_N,'RES) proc \<Rightarrow> ('ret,'RES_N,'RES) p
   where \<open>op_try f g s = (case f s of Success x s' \<Rightarrow> Success x s' | Exception s' \<Rightarrow> g s'
                                    | PartialCorrect \<Rightarrow> PartialCorrect | Fail \<Rightarrow> Fail)\<close>
 
-lemma (in \<phi>min) "__op_try__":
+lemma (in \<phi>empty) "__op_try__":
   \<open> \<^bold>p\<^bold>r\<^bold>o\<^bold>c f \<lbrace> X \<longmapsto> Y1 \<^bold>t\<^bold>h\<^bold>r\<^bold>o\<^bold>w\<^bold>s E \<rbrace>
 \<Longrightarrow> \<^bold>p\<^bold>r\<^bold>o\<^bold>c g \<lbrace> E \<longmapsto> Y2 \<^bold>t\<^bold>h\<^bold>r\<^bold>o\<^bold>w\<^bold>s E2 \<rbrace>
 \<Longrightarrow> \<^bold>p\<^bold>r\<^bold>o\<^bold>c op_try f g \<lbrace> X \<longmapsto> \<lambda>v. Y1 v + Y2 v \<^bold>t\<^bold>h\<^bold>r\<^bold>o\<^bold>w\<^bold>s E2 \<rbrace> \<close>
@@ -53,9 +53,7 @@ fn (ctxt,sequent) =>
 
 declare [ [\<phi>not_define_new_const] ]
 
-declare [ [\<phi>trace_processing] ]
-
-proc (in \<phi>min) try'':
+proc (in \<phi>empty) try'':
   assumes F: \<open>\<^bold>p\<^bold>r\<^bold>o\<^bold>c f \<lbrace> X \<longmapsto> YY \<^bold>t\<^bold>h\<^bold>r\<^bold>o\<^bold>w\<^bold>s E \<rbrace>\<close>
   assumes G: \<open>\<^bold>p\<^bold>r\<^bold>o\<^bold>c g \<lbrace> E \<longmapsto> YY \<^bold>t\<^bold>h\<^bold>r\<^bold>o\<^bold>w\<^bold>s EE2 \<rbrace>\<close>
   argument X
@@ -63,7 +61,7 @@ proc (in \<phi>min) try'':
   throws EE2
   \<medium_left_bracket> ;; "__op_try__"  ;; F G \<medium_right_bracket>. .
 
-proc (in \<phi>min) try':
+proc (in \<phi>empty) try':
   assumes A: \<open>Union_the_Same_Or_Arbitrary_when_Var Z Y1 Y2\<close>
   assumes F: \<open>\<^bold>p\<^bold>r\<^bold>o\<^bold>c f \<lbrace> X \<longmapsto> Y1 \<^bold>t\<^bold>h\<^bold>r\<^bold>o\<^bold>w\<^bold>s E \<rbrace>\<close>
   assumes G: \<open>\<^bold>p\<^bold>r\<^bold>o\<^bold>c g \<lbrace> E \<longmapsto> Y2 \<^bold>t\<^bold>h\<^bold>r\<^bold>o\<^bold>w\<^bold>s E2 \<rbrace>\<close>
@@ -75,115 +73,6 @@ proc (in \<phi>min) try':
   \<medium_right_bracket>. .
 
 declare [ [\<phi>not_define_new_const = false] ]
-
-
-subsection \<open>Arithmetic Operations\<close>
-
-subsubsection \<open>Integer arithmetic\<close>
-
-definition op_const_int :: "nat \<Rightarrow> nat \<Rightarrow> ('VAL,'RES_N,'RES) proc"
-  where "op_const_int bits const = Success (sem_value (V_int.mk (bits,const)))"
-
-definition op_const_size_t :: "nat \<Rightarrow> ('VAL,'RES_N,'RES) proc"
-  where "op_const_size_t c = \<phi>M_assume (c < 2 ^ addrspace_bits)
-                          \<ggreater> Success (sem_value (V_int.mk (addrspace_bits,c)))"
-  \<comment> \<open> `op_const_size_t` checks the overflow during the compilation towards certain decided platform.  \<close>
-
-definition op_add :: "nat \<Rightarrow> ('VAL \<times> 'VAL, 'VAL, 'RES_N, 'RES) proc'"
-  where "op_add bits =
-      \<phi>M_caseV (\<lambda>va vb.
-      \<phi>M_getV (\<tau>Int bits) (snd o V_int.dest) va (\<lambda>val_a.
-      \<phi>M_getV (\<tau>Int bits) (snd o V_int.dest) vb (\<lambda>val_b.
-      Success (sem_value (V_int.mk (bits, ((val_a + val_b) mod 2^bits))))
-  )))"
-
-
-(* lemma (in \<phi>min) op_add:
-  \<open> \<^bold>p\<^bold>r\<^bold>e\<^bold>m\<^bold>i\<^bold>s\<^bold>e x + y < 2^b
-\<Longrightarrow> \<^bold>p\<^bold>r\<^bold>o\<^bold>c op_add b (\<phi>V_pair vb va) \<lbrace> x \<Ztypecolon> Val va \<nat>[b]\<heavy_comma> y \<Ztypecolon> Val vb \<nat>[b] \<longmapsto> \<^bold>v\<^bold>a\<^bold>l x + y \<Ztypecolon> \<nat>[b] \<rbrace>\<close>
-  unfolding op_add_def Premise_def
-  by (cases va; cases vb; simp, \<phi>reason) *)
-
-
-(* lemma (in \<phi>min)
-  \<open> \<^bold>p\<^bold>r\<^bold>o\<^bold>c left  \<lbrace> R1 \<longmapsto> R2\<heavy_comma> SYNTHESIS x \<Ztypecolon> \<nat>[b] \<rbrace>
-\<Longrightarrow> \<^bold>p\<^bold>r\<^bold>o\<^bold>c right \<lbrace> R2 \<longmapsto> R3\<heavy_comma> SYNTHESIS y \<Ztypecolon> \<nat>[b] \<rbrace>
-\<Longrightarrow> \<^bold>p\<^bold>r\<^bold>e\<^bold>m\<^bold>i\<^bold>s\<^bold>e x + y < 2^b
-\<Longrightarrow> \<^bold>p\<^bold>r\<^bold>o\<^bold>c (left \<ggreater> right \<ggreater> op_add b) \<lbrace> R1 \<longmapsto> R3\<heavy_comma> SYNTHESIS x + y \<Ztypecolon> \<nat>[b] \<rbrace>\<close>
-  apply (\<phi>reason, assumption) *)
-
-definition op_sub :: "nat \<Rightarrow> ('VAL \<times> 'VAL, 'VAL, 'RES_N, 'RES) proc'"
-  where "op_sub bits =
-      \<phi>M_caseV (\<lambda>va vb.
-      \<phi>M_getV (\<tau>Int bits) (snd o V_int.dest) va (\<lambda>val_a.
-      \<phi>M_getV (\<tau>Int bits) (snd o V_int.dest) vb (\<lambda>val_b.
-      Success (sem_value (V_int.mk (bits, ((2^bits + val_b - val_a) mod 2^bits))))
-  )))"
-
-definition op_umul :: "nat \<Rightarrow> ('VAL \<times> 'VAL, 'VAL, 'RES_N, 'RES) proc'"
-  where "op_umul bits =
-      \<phi>M_caseV (\<lambda>va vb.
-      \<phi>M_getV (\<tau>Int bits) (snd o V_int.dest) va (\<lambda>val_a.
-      \<phi>M_getV (\<tau>Int bits) (snd o V_int.dest) vb (\<lambda>val_b.
-      Success (sem_value (V_int.mk (bits, ((val_b * val_a) mod 2^bits))))
-  )))"
-
-definition op_udiv :: "nat \<Rightarrow> ('VAL \<times> 'VAL, 'VAL, 'RES_N, 'RES) proc'"
-  where "op_udiv bits =
-      \<phi>M_caseV (\<lambda>va vb.
-      \<phi>M_getV (\<tau>Int bits) (snd o V_int.dest) va (\<lambda>val_a.
-      \<phi>M_getV (\<tau>Int bits) (snd o V_int.dest) vb (\<lambda>val_b.
-      Success (sem_value (V_int.mk (bits, (val_b div val_a))))
-  )))"
-
-definition op_lt :: "nat \<Rightarrow> ('VAL \<times> 'VAL, 'VAL,'RES_N,'RES) proc'"
-  where "op_lt bits =
-      \<phi>M_caseV (\<lambda>va vb.
-      \<phi>M_getV (\<tau>Int bits) (snd o V_int.dest) va (\<lambda>val_a.
-      \<phi>M_getV (\<tau>Int bits) (snd o V_int.dest) vb (\<lambda>val_b.
-      Success (sem_value (V_int.mk (1, (if val_b < val_a then 1 else 0))))
-  )))"
-
-
-definition op_le :: "nat \<Rightarrow> ('VAL \<times> 'VAL, 'VAL,'RES_N,'RES) proc'"
-  where "op_le bits =
-      \<phi>M_caseV (\<lambda>va vb.
-      \<phi>M_getV (\<tau>Int bits) (snd o V_int.dest) va (\<lambda>val_a.
-      \<phi>M_getV (\<tau>Int bits) (snd o V_int.dest) vb (\<lambda>val_b.
-      Success (sem_value (V_int.mk (1, (if val_b \<le> val_a then 1 else 0))))
-  )))"
-
-
-definition op_not :: "('VAL, 'VAL,'RES_N,'RES) proc'"
-  where "op_not v =
-    \<phi>M_getV (\<tau>Int 1) (snd o V_int.dest) v (\<lambda>v.
-    Success (sem_value (V_int.mk (1, 1 - v)))
-  )"
-
-definition op_and :: "('VAL \<times> 'VAL, 'VAL,'RES_N,'RES) proc'"
-  where "op_and =
-    \<phi>M_caseV (\<lambda>va vb.
-    \<phi>M_getV (\<tau>Int 1) (snd o V_int.dest) va (\<lambda>v.
-    \<phi>M_getV (\<tau>Int 1) (snd o V_int.dest) vb (\<lambda>u.
-    Success (sem_value (V_int.mk (1, v+u-1)))
-  )))"
-
-definition op_or :: "('VAL \<times> 'VAL, 'VAL,'RES_N,'RES) proc'"
-  where "op_or =
-    \<phi>M_caseV (\<lambda>va vb.
-    \<phi>M_getV (\<tau>Int 1) (snd o V_int.dest) va (\<lambda>v.
-    \<phi>M_getV (\<tau>Int 1) (snd o V_int.dest) vb (\<lambda>u.
-    Success (sem_value (V_int.mk (1, min 1 (v+u))))
-  )))"
-
-definition op_equal :: "'TY \<Rightarrow> ('VAL \<times> 'VAL, 'VAL,'RES_N,'RES) proc'"
-  where "op_equal TY =
-    \<phi>M_caseV (\<lambda>va vb.
-    \<phi>M_getV TY id va (\<lambda>v.
-    \<phi>M_getV TY id vb (\<lambda>u.
-    (\<lambda>res. \<phi>M_assert (Can_EqCompare res u v) res) \<ggreater>
-    Success (sem_value (V_int.mk (1, (if EqCompare u v then 1 else 0))))
-)))"
 
 
 subsection \<open>Access the Resource\<close>
@@ -329,225 +218,7 @@ lemma (in mapping_resource) \<phi>R_allocate_res_entry[\<phi>reason!]:
 
 
 
-subsubsection \<open>Variable Operations\<close>
-
-definition \<phi>M_get_var :: "varname \<Rightarrow> 'TY \<Rightarrow> ('VAL \<Rightarrow> ('ret,'RES_N,'RES) proc) \<Rightarrow> ('ret,'RES_N,'RES) proc"
-  where "\<phi>M_get_var vname TY F = \<phi>M_get_res_entry (R_var.get) vname (\<lambda>val.
-            \<phi>M_assert (val \<in> Well_Type TY) \<ggreater> F val)"
-
-definition op_get_var :: "varname \<Rightarrow> 'TY \<Rightarrow> ('VAL,'RES_N,'RES) proc"
-  where "op_get_var vname TY = \<phi>M_get_var vname TY (\<lambda>x. Success (sem_value x))"
-
-definition op_set_var :: "varname \<Rightarrow> 'TY \<Rightarrow> ('VAL, unit, 'RES_N, 'RES) proc'"
-  where "op_set_var vname TY v =
-          \<phi>M_getV TY id v (\<lambda>v.
-          \<phi>M_get_var vname TY (\<lambda>_.
-          \<phi>M_set_res R_var.updt (\<lambda>f. f(vname := Some v))))"
-
-definition op_free_var :: "varname \<Rightarrow> (unit,'RES_N,'RES) proc"
-  where "op_free_var vname = \<phi>M_set_res R_var.updt (\<lambda>f. f(vname := None))"
-
-definition op_var_scope' :: "'TY
-                          \<Rightarrow> (varname \<Rightarrow> ('ret,'RES_N,'RES) proc)
-                          \<Rightarrow> ('VAL,'ret,'RES_N,'RES) proc'"
-  where "op_var_scope' TY F v =
-    \<phi>M_getV TY id v (\<lambda>v.
-    \<phi>M_get_res R_var.get (\<lambda>f.
-    let vname = (@vname. f vname = None) in
-    \<phi>M_set_res R_var.updt (\<lambda>f. f(vname := Some v)) \<ggreater>
-    F vname
-  ))"
-
-lemma (in \<phi>min) \<phi>M_get_var[\<phi>reason!]:
-  \<open>v \<in> Well_Type TY
-    \<Longrightarrow> \<^bold>p\<^bold>r\<^bold>o\<^bold>c F v \<lbrace> v \<Ztypecolon> Var vname Identity \<longmapsto> Y \<rbrace>
-    \<Longrightarrow> \<^bold>p\<^bold>r\<^bold>o\<^bold>c \<phi>M_get_var vname TY F \<lbrace> v \<Ztypecolon> Var vname Identity \<longmapsto> Y \<rbrace>\<close>
-  unfolding \<phi>Procedure_def \<phi>M_get_var_def \<phi>M_get_res_entry_def \<phi>M_get_res_def
-  apply (simp add: \<phi>expns R_var.prj.homo_mult times_list_def)
-  apply (subst R_var_valid_split)
-  apply (auto simp add: \<phi>expns FIC_var_split times_set_def R_var.mult_in_dom mult_strip_fine_011 times_fine times_list_def)
-  subgoal premises prems for R fic res vars
-  proof -
-    note [simp] = \<open>vars ## 1(vname \<mapsto> v)\<close> [THEN sep_disj_fun[where x=vname], simplified]
-    note F = \<open>\<forall>_ _. _ \<longrightarrow> F v _ \<in> _\<close>[THEN spec[where x=\<open>res * R_var.mk (Fine (1(vname \<mapsto> v)))\<close>],
-                                       THEN spec[where x=R], THEN mp]
-    show ?thesis
-      apply (simp add: times_fun)
-      apply (rule \<phi>M_assert', rule \<open>v \<in> Well_Type TY\<close>, rule F,
-             rule exI[where x=\<open>fic * FIC_var.mk (Fine (1(vname \<mapsto> v)))\<close>])
-      using prems apply (auto simp add: FIC_var_split times_set_def)
-      apply (subst R_var_valid_split)
-      apply (auto simp add: R_var.inj_homo_mult[symmetric] times_fine)
-      done
-  qed
-  done
-
-lemma (in \<phi>min) \<phi>M_set_var[\<phi>reason!]:
-  \<open>\<^bold>p\<^bold>r\<^bold>o\<^bold>c \<phi>M_set_res R_var.updt (\<lambda>f. f(vname \<mapsto> u)) \<lbrace> v \<Ztypecolon> Var vname Identity \<longmapsto> \<lambda>_. u \<Ztypecolon> Var vname Identity \<rbrace>\<close>
-  unfolding \<phi>M_set_res_def \<phi>Procedure_def
-  apply (auto simp add: \<phi>expns R_var_valid_split' R_var.prj.homo_mult FIC_var_split
-                        R_var.mult_in_dom mult_strip_fine_011 times_list_def)
-  subgoal premises prems for R fic res vars
-  proof -
-    note [simp] = \<open>vars ## 1(vname \<mapsto> v)\<close> [THEN sep_disj_fun[where x=vname], simplified]
-    have [simp]: \<open>(vars * 1(vname \<mapsto> v))(vname \<mapsto> u) = vars * 1(vname \<mapsto> u)\<close>
-      unfolding times_fun_def fun_eq_iff fun_upd_def by simp
-    from \<open>vars ## 1(vname \<mapsto> v)\<close> have [simp]: \<open>vars ## 1(vname \<mapsto> u)\<close>
-      unfolding sep_disj_fun_def by simp
-    show ?thesis
-      apply (rule exI[where x=\<open>fic * FIC_var.mk (Fine (1(vname \<mapsto> u))) \<close>])
-      apply (auto simp add: R_var_valid_split' FIC_var_split times_set_def prems)
-      apply (rule exI[where x = res])
-      by (auto simp add: fun_eq_iff times_fun prems R_var.inj_homo_mult[symmetric] times_fine)
-  qed
-  done
-
-
-lemma (in \<phi>min) op_get_var''_\<phi>app:
-   \<open>\<^bold>p\<^bold>r\<^bold>e\<^bold>m\<^bold>i\<^bold>s\<^bold>e v \<in> Well_Type TY
-    \<Longrightarrow> \<^bold>p\<^bold>r\<^bold>o\<^bold>c op_get_var vname TY \<lbrace> v \<Ztypecolon> Var vname Identity \<longmapsto> v \<Ztypecolon> Var vname Identity \<heavy_comma> \<^bold>v\<^bold>a\<^bold>l v \<Ztypecolon> Identity \<rbrace>\<close>
-  unfolding op_get_var_def Premise_def
-  by (\<phi>reason, assumption, \<phi>reason)
-end
-
-
-lemma (in \<phi>min) op_set_var''_\<phi>app:
-   \<open>\<^bold>p\<^bold>r\<^bold>e\<^bold>m\<^bold>i\<^bold>s\<^bold>e v \<in> Well_Type TY
-\<Longrightarrow> \<^bold>p\<^bold>r\<^bold>e\<^bold>m\<^bold>i\<^bold>s\<^bold>e u \<in> Well_Type TY
-\<Longrightarrow> \<^bold>p\<^bold>r\<^bold>o\<^bold>c op_set_var vname TY rawv \<lbrace> v \<Ztypecolon> Var vname Identity\<heavy_comma> u \<Ztypecolon> Val rawv Identity \<longmapsto> u \<Ztypecolon> Var vname Identity \<rbrace>\<close>
-  unfolding op_set_var_def Premise_def
-  by (cases rawv; simp, \<phi>reason, assumption, simp add: \<phi>expns, \<phi>reason)
-
-
-lemma (in \<phi>min) op_var_scope':
-   \<open>\<^bold>p\<^bold>r\<^bold>e\<^bold>m\<^bold>i\<^bold>s\<^bold>e v \<in> Well_Type TY
-    \<Longrightarrow> (\<And>vname. \<^bold>p\<^bold>r\<^bold>o\<^bold>c F vname \<lbrace> X\<heavy_comma> v \<Ztypecolon> Var vname Identity \<longmapsto> Y \<^bold>t\<^bold>h\<^bold>r\<^bold>o\<^bold>w\<^bold>s E \<rbrace> )
-    \<Longrightarrow> \<^bold>p\<^bold>r\<^bold>o\<^bold>c op_var_scope' TY F rawv \<lbrace> X\<heavy_comma> v \<Ztypecolon> Val rawv Identity \<longmapsto> Y \<^bold>t\<^bold>h\<^bold>r\<^bold>o\<^bold>w\<^bold>s E \<rbrace>\<close>
-  unfolding op_var_scope'_def Premise_def
-  apply (cases rawv; simp, \<phi>reason, simp add: \<phi>expns)
-  unfolding \<phi>Procedure_def
-  unfolding \<phi>M_set_res_def \<phi>Procedure_def \<phi>M_get_res_def Let_def bind_def
-  apply (simp add: \<phi>expns)
-  apply (auto simp add: \<phi>expns R_var_valid_split' R_var.prj.homo_mult FIC_var_split
-                        R_var.mult_in_dom mult_strip_fine_011 times_list_def)
-  subgoal premises prems for res R ficR ficX vars
-  proof -
-    note t1 = finite_map_freshness[OF \<open>finite (dom vars)\<close>, OF infinite_varname]
-    have t2[simp]: \<open>vars ## 1(SOME fic. vars fic = None \<mapsto> v)\<close>
-      unfolding sep_disj_fun_def by simp (meson someI t1)
-    have t3[simp]: \<open>vars (SOME vname. vars vname = None) = None\<close>
-      by (meson someI t1)
-    show ?thesis
-      apply (rule \<open>\<forall>a. _\<close>[of \<open>(SOME vname. vars vname = None)\<close>,
-        THEN spec, THEN spec, THEN mp])
-      apply (rule exI[where x=\<open>ficR * ficX * FIC_var.mk (Fine (1((@x. vars x = None) \<mapsto> v))) \<close>])
-      apply (auto simp add: \<phi>expns R_var_valid_split' FIC_var_split times_set_def prems)
-      using \<open>ficR \<in> R\<close> \<open>ficX \<in> X\<close> apply (smt (verit) fun_mult_norm) 
-      apply (rule exI[where x = res])
-      by (simp add: fun_eq_iff times_fun prems R_var.inj_homo_mult[symmetric] times_fine)
-  qed
-  done
-
-lemma (in \<phi>min) op_free_var:
-   \<open>\<^bold>p\<^bold>r\<^bold>o\<^bold>c op_free_var vname \<lbrace> v \<Ztypecolon> Var vname Identity \<longmapsto> 1 \<rbrace>\<close>
-  unfolding op_free_var_def \<phi>Procedure_def \<phi>M_set_res_def
-  apply (auto simp add: \<phi>expns R_var_valid_split' R_var.prj.homo_mult FIC_var_split
-                        R_var.mult_in_dom mult_strip_fine_011 times_list_def)
-  subgoal premises prems for R fic res vars
-  proof -
-    note [simp] = \<open>vars ## 1(vname \<mapsto> v)\<close> [THEN sep_disj_fun[where x=vname], simplified]
-    have [simp]: \<open>(vars * 1(vname \<mapsto> v))(vname := None) = vars\<close>
-      unfolding fun_upd_def fun_eq_iff times_fun by simp
-    have [simp]: \<open>(res * R_var.mk (Fine (1(vname \<mapsto> v))))(R_var.name := R_var.inject (Fine vars)) = res\<close>
-      by (simp add: times_fun_def fun_upd_def fun_eq_iff prems)
-    show ?thesis
-      apply (rule exI[where x=fic])
-      by (auto simp add: prems)
-  qed
-  done
-
-
-
-
-
-
-context \<phi>min begin
-
-
-
-
-
-
-
-subsection \<open>Branches & Loops\<close>
-
-paragraph \<open>Non-Branching Selection\<close>
-
-definition op_sel :: "'TY \<Rightarrow> ('VAL \<times> 'VAL \<times> 'VAL, 'VAL,'RES_N,'RES) proc'"
-  where "op_sel TY =
-    \<phi>M_caseV (\<lambda>vc. \<phi>M_caseV (\<lambda>va vb.
-    \<phi>M_getV (\<tau>Int 1) V_int.dest vc (\<lambda>c.
-    \<phi>M_getV TY id va (\<lambda>a.
-    \<phi>M_getV TY id vb (\<lambda>b.
-    Success (sem_value (if snd c = 1 then b else a)))))))"
-
-paragraph \<open>Branch\<close>
-
-definition op_if :: "('ret,'RES_N,'RES) proc
-                  \<Rightarrow> ('ret,'RES_N,'RES) proc
-                  \<Rightarrow> ('VAL,'ret,'RES_N,'RES) proc'"
-  where "op_if brT brF v =
-    \<phi>M_getV (\<tau>Int 1) V_int.dest v (\<lambda>c. (if snd c = 1 then brT else brF))"
-
-paragraph \<open>While Loop\<close>
-
-inductive SemDoWhile :: "('VAL,'RES_N,'RES) proc \<Rightarrow> ('RES_N \<Rightarrow> 'RES) \<Rightarrow> (unit,'RES_N,'RES) state \<Rightarrow> bool" where
-  "f s = Success (sem_value (V_int.mk (1,0))) res \<Longrightarrow> SemDoWhile f s (Success (sem_value ()) res)"
-| "f s = Success (sem_value (V_int.mk (1,1))) res \<Longrightarrow> SemDoWhile f res s'' \<Longrightarrow> SemDoWhile f s s''"
-| "f s = Exception e \<Longrightarrow> SemDoWhile f s (Exception e)"
-| "f s = PartialCorrect \<Longrightarrow> SemDoWhile f s PartialCorrect"
-| "f s = Fail \<Longrightarrow> SemDoWhile f s Fail"
-
-lemma "\<nexists> y. SemDoWhile (\<lambda>res. Success (sem_value (V_int.mk (1,1))) res) res y"
-  apply rule apply (elim exE) subgoal for y 
-    thm SemDoWhile.induct
-    apply (induct "(\<lambda>res. Success (sem_value (V_int.mk (1,1))) (res::'RES_N \<Rightarrow> 'RES))" res y
-           rule: SemDoWhile.induct)
-       apply simp_all
-    done done
-
-definition op_do_while :: "('VAL,'RES_N,'RES) proc \<Rightarrow> (unit,'RES_N,'RES) proc" where
-  "op_do_while f s = (if (\<exists>y. SemDoWhile f s y) then The (SemDoWhile f s) else PartialCorrect)"
-
-lemma SemDoWhile_deterministic:
-  assumes "SemDoWhile c s s1"
-      and "SemDoWhile c s s2"
-    shows "s1 = s2"
-proof -
-  have "SemDoWhile c s s1 \<Longrightarrow> (\<forall>s2. SemDoWhile c s s2 \<longrightarrow> s1 = s2)"
-    apply (induct rule: SemDoWhile.induct)
-    by (subst SemDoWhile.simps, simp)+
-  thus ?thesis
-    using assms by simp
-qed
-
-lemma SemDoWhile_deterministic2:
-    "SemDoWhile body s x \<Longrightarrow> The ( SemDoWhile body s) = x"
-  using SemDoWhile_deterministic by blast
-
-
-paragraph \<open>Recursion\<close>
-
-inductive SemRec :: "(('a,'a,'RES_N,'RES) proc' \<Rightarrow> ('a,'a,'RES_N,'RES) proc')
-            \<Rightarrow> 'a sem_value \<Rightarrow> ('RES_N \<Rightarrow> 'RES) \<Rightarrow> ('a,'RES_N,'RES) state \<Rightarrow> bool"
-where
-  SemRec_I0: "(\<And>g. F g x res = y) \<Longrightarrow> SemRec F x res y"
-| SemRec_IS: "SemRec (F o F) x res y \<Longrightarrow> SemRec F x res y"
-
-definition op_recursion :: "'TY list \<Rightarrow> 'TY list
-                         \<Rightarrow> (('a,'a,'RES_N,'RES) proc' \<Rightarrow> ('a,'a,'RES_N,'RES) proc')
-                         \<Rightarrow> ('a,'a,'RES_N,'RES) proc'"
-  where "op_recursion _ _ F x s = (if (\<exists>t. SemRec F x s t) then The (SemRec F x s) else PartialCorrect)"
+(*
 
 
 (*
@@ -586,11 +257,11 @@ lemma cons_tup_cons:
   apply (smt (verit, del_insts) Suc_le_eq append1_eq_conv list.sel(1) list_all2_Cons2 rev_eq_Cons_iff take_hd_drop)
   by (simp add: take_Suc_conv_app_nth)
 
-lemma (in \<phi>min) op_cons_tup_nil:
+lemma (in \<phi>empty) op_cons_tup_nil:
   \<open> \<^bold>p\<^bold>r\<^bold>o\<^bold>c cons_tup [] \<lbrace> Void \<longmapsto> () \<Ztypecolon> EmptyTuple \<rbrace>\<close>
   unfolding cons_tup_nil by \<phi>reason
 
-lemma (in \<phi>min) op_cons_tup_cons:
+lemma (in \<phi>empty) op_cons_tup_cons:
   \<open> \<^bold>p\<^bold>r\<^bold>o\<^bold>c cons_tup TYs \<lbrace> X \<longmapsto> VAL y \<Ztypecolon> Y \<rbrace>
 \<Longrightarrow> \<phi>SemType (a \<Ztypecolon> A) TY
 \<Longrightarrow> \<^bold>p\<^bold>r\<^bold>o\<^bold>c cons_tup (TY#TYs) \<lbrace> VAL a \<Ztypecolon> A\<heavy_comma> X \<longmapsto> VAL (a,y) \<Ztypecolon> (\<clubsuit> A \<^emph> Y) \<rbrace>\<close>
@@ -626,11 +297,11 @@ lemma op_dest_tup_cons_expn:
       instr_comp_def bind_def)
   by (metis list.discI list.exhaust_sel list.rel_sel list.sel(1))
 
-lemma (in \<phi>min) op_dest_tup_nil:
+lemma (in \<phi>empty) op_dest_tup_nil:
   \<open>\<^bold>p\<^bold>r\<^bold>o\<^bold>c op_dest_tup [] \<lbrace> () \<Ztypecolon> EmptyTuple \<longmapsto> Void \<rbrace> \<close>
   unfolding op_dest_tup_nil_expn by \<phi>reason
 
-lemma (in \<phi>min) op_dest_tup_cons:
+lemma (in \<phi>empty) op_dest_tup_cons:
   \<open> \<^bold>p\<^bold>r\<^bold>o\<^bold>c op_dest_tup TYs \<lbrace> VAL y \<Ztypecolon> Y \<longmapsto> X \<rbrace>
 \<Longrightarrow> \<phi>SemType (a \<Ztypecolon> A) TY
 \<Longrightarrow> \<^bold>p\<^bold>r\<^bold>o\<^bold>c op_dest_tup (TY#TYs) \<lbrace> VAL (a,y) \<Ztypecolon> (\<clubsuit> A \<^emph> \<phi>Is_Tuple Y) \<longmapsto> VAL a \<Ztypecolon> A\<heavy_comma> X \<rbrace>\<close>
@@ -659,7 +330,7 @@ definition op_set_element :: "nat list \<Rightarrow> 'TY \<Rightarrow> ('VAL,'RE
     \<phi>M_put_Val (index_mod_value idx (\<lambda>_. u) v)
   ))"
 
-lemma (in \<phi>min) op_get_element:
+lemma (in \<phi>empty) op_get_element:
   \<open> \<^bold>s\<^bold>i\<^bold>m\<^bold>p\<^bold>r\<^bold>e\<^bold>m valid_index TY idx
 \<Longrightarrow> \<phi>SemType (x \<Ztypecolon> X) TY
 \<Longrightarrow> \<phi>Index_getter idx X Y f
@@ -668,7 +339,7 @@ lemma (in \<phi>min) op_get_element:
   apply \<phi>reason apply (simp add: \<phi>SemType_def subset_iff)
   by \<phi>reason
 
-lemma (in \<phi>min) op_set_element:
+lemma (in \<phi>empty) op_set_element:
   \<open> \<^bold>s\<^bold>i\<^bold>m\<^bold>p\<^bold>r\<^bold>e\<^bold>m valid_index TY idx
 \<Longrightarrow> \<phi>Index_mapper idx X Y f
 \<Longrightarrow> \<phi>SemType (x \<Ztypecolon> X) TY
@@ -682,7 +353,7 @@ lemma (in \<phi>min) op_set_element:
 
 *)
 
-
+*)
 
 end
 
