Phi_Min.thy
@@ -1,0 +1,628 @@
+theory Phi_Min
+  imports NuSys NuInstructions
+begin
+
+chapter \<open>Minimal Semantics\<close>
+
+text \<open>This minimal semantics contains integer and variable.\<close>
+
+section \<open>Semantic\<close>
+
+subsection \<open>Models\<close>
+
+subsubsection \<open>Type\<close>
+
+virtual_datatype \<phi>min_ty = \<phi>empty_ty +
+  T_int     :: nat \<comment> \<open>in unit of bits\<close>
+
+context \<phi>min_ty begin
+abbreviation \<open>\<tau>Int \<equiv> T_int.mk\<close>
+end
+
+subsubsection \<open>Value\<close>
+
+virtual_datatype 'TY \<phi>min_val :: "nonsepable_semigroup" = 'TY \<phi>empty_val +
+  V_int     :: \<open>nat \<times> nat\<close>
+
+subsubsection \<open>Resource\<close>
+
+typedef varname = \<open>UNIV::nat set\<close> ..
+type_synonym ('TY,'VAL) R_var = \<open>(varname \<rightharpoonup> 'VAL) ?\<close>
+
+lemma infinite_varname:
+  \<open>infinite (UNIV::varname set)\<close>
+  by (metis (mono_tags, opaque_lifting) Rep_varname_cases UNIV_I finite_imageI infinite_UNIV_char_0 surj_def)
+
+resource_space ('VAL::"nonsepable_semigroup",'TY) \<phi>min_res = ('VAL,'TY) \<phi>empty_res +
+  R_var :: \<open>('TY,'VAL) R_var\<close>
+
+subsubsection \<open>Pure Semantics\<close>
+
+locale \<phi>min_sem =
+  \<phi>empty_sem where TYPES = TYPES
++ \<phi>min_ty  where CONS_OF   = TY_CONS_OF
+            and TYPE'NAME = \<open>TYPE('TY_N)\<close>
+            and TYPE'REP  = \<open>TYPE('TY)\<close>
++ \<phi>min_val where CONS_OF   = VAL_CONS_OF
+            and TYPE'TY   = \<open>TYPE('TY)\<close>
+            and TYPE'NAME = \<open>TYPE('VAL_N)\<close>
+            and TYPE'REP  = \<open>TYPE('VAL::nonsepable_semigroup)\<close>
++ \<phi>min_res where TYPE'VAL  = \<open>TYPE('VAL)\<close>
+            and TYPE'TY   = \<open>TYPE('TY)\<close>
+            and TYPE'NAME = \<open>TYPE('RES_N)\<close>
+            and TYPE'REP  = \<open>TYPE('RES::{no_inverse,comm_monoid_mult})\<close>
++ \<phi>resource_sem where Resource_Validator = Resource_Validator
++ \<phi>resource_sem where Resource_Validator = Resource_Validator
+for TYPES :: \<open>(('TY_N \<Rightarrow> 'TY)
+                \<times> ('VAL_N => 'VAL::nonsepable_semigroup)
+                \<times> ('RES_N => 'RES::{comm_monoid_mult,no_inverse})) itself\<close>
++
+assumes WT_int[simp]: \<open>Well_Type (\<tau>Int b)     = { V_int.mk (b,x)    |x. x < 2^b } \<close>
+assumes res_valid_var[simp]: \<open>Resource_Validator R_var.name = {R_var.inject (Fine vars) |vars. finite (dom vars)}\<close>
+assumes can_eqcmp_int[simp]: "Can_EqCompare res (V_int.mk (b1,x1)) (V_int.mk (b2,x2)) \<longleftrightarrow> b1 = b2"
+assumes eqcmp_int[simp]: "EqCompare (V_int.mk i1) (V_int.mk i2) \<longleftrightarrow> i1 = i2"
+assumes zero_int[simp]: \<open>Zero (T_int.mk b)      = V_int.mk (b,0)\<close>
+
+begin
+
+lemma Valid_Types[simp]:
+  \<open>Valid_Type (\<tau>Int n)\<close>
+  unfolding Inhabited_def
+  apply (simp)
+  using less_exp by blast
+
+sublocale R_var: partial_map_resource \<open>{vars. finite (dom vars)}\<close> R_var
+  by (standard; simp add: set_eq_iff image_iff; blast)
+
+end
+
+fiction_space (in \<phi>min_sem) \<phi>min_fic :: \<open>'RES_N \<Rightarrow> 'RES\<close> =
+  FIC_var :: \<open>R_var.basic_fine_fiction (fiction.fine fiction.it)\<close>
+
+locale \<phi>min =
+  \<phi>min_fic where TYPES = \<open>TYPE(('TY_N \<Rightarrow> 'TY) \<times> ('VAL_N \<Rightarrow> 'VAL::nonsepable_semigroup)
+                            \<times> ('RES_N \<Rightarrow> 'RES::{no_inverse,comm_monoid_mult}))\<close>
+    and TYPE'NAME = \<open>TYPE('FIC_N)\<close>
+    and TYPE'REP = \<open>TYPE('FIC::{no_inverse,comm_monoid_mult})\<close> 
++ \<phi>empty where TYPES = \<open>TYPE(('TY_N \<Rightarrow> 'TY)
+                          \<times> ('VAL_N \<Rightarrow> 'VAL::nonsepable_semigroup)
+                          \<times> ('RES_N \<Rightarrow> 'RES::{no_inverse,comm_monoid_mult})
+                          \<times> ('FIC_N \<Rightarrow> 'FIC))\<close>
++ fixes TYPES :: \<open>(('TY_N \<Rightarrow> 'TY) \<times> ('VAL_N \<Rightarrow> 'VAL) \<times> ('RES_N \<Rightarrow> 'RES) \<times> ('FIC_N \<Rightarrow> 'FIC)) itself\<close>
+begin
+
+sublocale FIC_var: identity_fiction_for_fine_resource \<open>{vars. finite (dom vars)}\<close> R_var
+    Resource_Validator INTERPRET FIC_var ..
+
+end
+
+section \<open>\<phi>-Types\<close>
+
+context \<phi>min begin
+
+subsection \<open>Integer\<close>
+
+\<phi>overloads nat and int
+
+subsubsection \<open>Natural Nmbers\<close>
+
+paragraph \<open>Natural Number\<close>
+
+definition \<phi>Nat :: "nat \<Rightarrow> ('VAL, nat) \<phi>" ("\<nat>[_]")
+  where "\<nat>[b] x = (if x < 2^b then { V_int.mk (b,x) } else {})"
+
+abbreviation \<open>Size \<equiv> \<nat>[addrspace_bits]\<close>
+
+lemma \<phi>Nat_expn[\<phi>expns]:
+  "p \<in> (x \<Ztypecolon> \<nat>[b]) \<longleftrightarrow> (p = V_int.mk (b,x)) \<and> x < 2^b"
+  unfolding \<phi>Type_def by (simp add: \<phi>Nat_def)
+
+lemma \<phi>Nat_elim[elim!,\<phi>reason_elim!]:
+  "Inhabited (x \<Ztypecolon> \<nat>[b]) \<Longrightarrow> (x < 2^b \<Longrightarrow> C) \<Longrightarrow> C"
+  unfolding Inhabited_def by (auto simp add: \<phi>expns)
+
+lemma \<phi>Nat_semty[\<phi>reason on \<open>\<phi>SemType (?x \<Ztypecolon> \<nat>[?b]) ?ty\<close>]:
+  \<open>\<phi>SemType (x \<Ztypecolon> \<nat>[b]) (\<tau>Int b)\<close>
+  unfolding \<phi>SemType_def subset_iff by (simp add: \<phi>expns)
+
+lemma [\<phi>reason on \<open>\<phi>Equal (\<nat>[?b]) ?c ?eq\<close>]:
+  "\<phi>Equal (\<nat>[b]) (\<lambda>x y. True) (=)"
+  unfolding \<phi>Equal_def by (auto simp add: unsigned_word_eqI \<phi>expns)
+
+lemma [\<phi>reason on \<open>\<phi>Zero (T_int.mk ?b) (\<nat>[?b]) ?zero\<close>]:
+  "\<phi>Zero (T_int.mk b) (\<nat>[b]) 0" unfolding \<phi>Zero_def by (simp add: \<phi>expns)
+
+paragraph \<open>Rounded Natural Number\<close>
+
+definition \<phi>NatRound :: "nat \<Rightarrow> ('VAL, nat) \<phi>" ("\<nat>\<^sup>r[_]")
+  where "\<nat>\<^sup>r[b] x = { V_int.mk (b, (x mod 2^b)) }"
+
+lemma \<phi>NatRound_expn[\<phi>expns]:
+  "p \<in> (x \<Ztypecolon> \<nat>\<^sup>r[b]) \<longleftrightarrow> p = V_int.mk (b, (x mod 2^b))"
+  unfolding \<phi>Type_def \<phi>NatRound_def by simp
+
+lemma [\<phi>reason on \<open>\<phi>Zero (T_int.mk ?b) \<nat>\<^sup>r[?b] ?z\<close>]:
+  "\<phi>Zero (T_int.mk b) (\<nat>\<^sup>r[b]) 0"
+  unfolding \<phi>Zero_def by (simp add: \<phi>expns)
+
+lemma \<phi>NatRound_semty[\<phi>reason on \<open>\<phi>SemType (?x \<Ztypecolon> \<nat>\<^sup>r[?b]) ?ty\<close>]:
+  \<open>\<phi>SemType (x \<Ztypecolon> \<nat>\<^sup>r[b]) (\<tau>Int b)\<close>
+  unfolding \<phi>SemType_def subset_iff by (simp add: \<phi>expns)
+
+subsubsection \<open>Integer in the normal sense\<close>
+
+
+definition \<phi>Int :: "nat \<Rightarrow> ('VAL, int) \<phi>" ("\<int>[_]")
+  where "\<phi>Int b x =(if x < 2^(b - 1) \<and> -(2^(b-1)) \<le> x \<and> (b = 0 \<longrightarrow> x = 0)
+                    then { V_int.mk (b, (if x \<ge> 0 then nat x else nat (2^b + x))) }
+                    else {})"
+
+lemma \<phi>Int_expn[\<phi>expns]:
+  "p \<in> (x \<Ztypecolon> \<int>[b]) \<longleftrightarrow> p = V_int.mk (b, (if x \<ge> 0 then nat x else nat (2^b + x)))
+                      \<and> x < 2^(b - 1) \<and> -(2^(b-1)) \<le> x \<and> (b = 0 \<longrightarrow> x = 0)"
+  unfolding \<phi>Type_def by (simp add: \<phi>Int_def)
+
+lemma \<phi>Int_inhabited[elim!,\<phi>reason_elim!]:
+  "Inhabited (x \<Ztypecolon> \<int>[b]) \<Longrightarrow> (x < 2^(b - 1) \<and> -(2^(b-1)) \<le> x \<and> (b = 0 \<longrightarrow> x = 0) \<Longrightarrow> C) \<Longrightarrow> C"
+  unfolding Inhabited_def by (simp add: \<phi>expns) 
+
+
+lemma [simp]: \<open>- (2^(b - 1)) \<le> x \<Longrightarrow> 0 \<le> 2 ^ b + x\<close> for x :: int
+  by (smt (verit, best) diff_le_self power_increasing_iff)
+
+lemma [\<phi>reason on \<open>\<phi>Equal \<int>[b] ?c ?eq\<close>]:
+    "\<phi>Equal \<int>[b] (\<lambda>x y. True) (=)"
+  unfolding \<phi>Equal_def by (cases b) (auto simp add: \<phi>expns eq_nat_nat_iff)
+
+lemma [\<phi>reason on \<open>\<phi>Zero (T_int.mk ?b) \<int>[?b] ?x\<close>]:
+    "\<phi>Zero (T_int.mk b) \<int>[b] 0"
+  unfolding \<phi>Zero_def by (simp add: \<phi>expns)
+
+lemma \<phi>Int_semty[\<phi>reason on \<open>\<phi>SemType (?x \<Ztypecolon> \<int>[?b]) ?ty\<close>]:
+  \<open>\<phi>SemType (x \<Ztypecolon> \<int>[b]) (\<tau>Int b)\<close>
+  unfolding \<phi>SemType_def subset_iff
+  by (simp add: \<phi>expns) (smt (verit, ccfv_SIG) diff_le_self power_increasing_iff)
+
+
+subsubsection \<open>Subtyping\<close>
+
+lemma subty_Z_N[\<phi>overload nat]: 
+  "\<^bold>p\<^bold>r\<^bold>e\<^bold>m\<^bold>i\<^bold>s\<^bold>e 0 < x \<Longrightarrow> \<^bold>s\<^bold>u\<^bold>b\<^bold>t\<^bold>y\<^bold>p\<^bold>e x \<Ztypecolon> \<int>[b] \<longmapsto> nat x \<Ztypecolon> \<nat>[b]"
+  unfolding Subty_def Premise_def apply (simp add: \<phi>expns del: One_nat_def)
+  by (smt (verit, del_insts) diff_less less_numeral_extra(1) power_strict_increasing_iff)
+
+lemma subty_N_Z[\<phi>overload int]:
+  "\<^bold>p\<^bold>r\<^bold>e\<^bold>m\<^bold>i\<^bold>s\<^bold>e x < 2^(b - 1) \<Longrightarrow> \<^bold>s\<^bold>u\<^bold>b\<^bold>t\<^bold>y\<^bold>p\<^bold>e x \<Ztypecolon> \<nat>[b] \<longmapsto> int x \<Ztypecolon> \<int>[b]"
+  unfolding Subty_def Premise_def apply (simp add: \<phi>expns del: One_nat_def)
+  by (metis less_one linorder_le_cases neg_0_le_iff_le not_exp_less_eq_0_int of_nat_0_le_iff order_trans power_0)
+
+
+subsubsection \<open>Boolean\<close>
+
+(* lemma [simp]: "(x \<noteq> 1) = (x = 0)" for x :: "1 word" proof -
+  have "(UNIV:: 1 word set) = {0,1}" unfolding UNIV_word_eq_word_of_nat
+  using less_2_cases apply auto apply force
+  by (metis UNIV_I UNIV_word_eq_word_of_nat len_num1 power_one_right)
+  then show ?thesis  by auto
+qed *)
+
+definition \<phi>Bool :: "('VAL, bool) \<phi>" ("\<bool>")
+  where "\<bool> x = { V_int.mk (1, (if x then 1 else 0)) }"
+
+lemma \<phi>Bool_expn[\<phi>expns]:
+  " p \<in> (x \<Ztypecolon> \<bool>) \<longleftrightarrow> p = V_int.mk (1, (if x then 1 else 0))"
+  unfolding \<phi>Type_def \<phi>Bool_def by simp
+
+lemma \<phi>Bool_inhabited[\<phi>reason_elim, elim!]:
+  \<open>Inhabited (x \<Ztypecolon> \<bool>) \<Longrightarrow> C \<Longrightarrow> C\<close> .
+
+lemma \<phi>Bool_eqcmp[\<phi>reason on \<open>\<phi>Equal \<bool> ?c ?eq\<close>]:
+  "\<phi>Equal \<bool> (\<lambda>x y. True) (=)"
+  unfolding \<phi>Equal_def by (simp add: \<phi>expns)
+
+lemma \<phi>Bool_zero[\<phi>reason on \<open>\<phi>Zero (\<tau>Int 1) \<bool> ?z\<close>]:
+  "\<phi>Zero (\<tau>Int 1) \<bool> False"
+  unfolding \<phi>Zero_def by (simp add: \<phi>expns)
+
+lemma \<phi>Bool_semty[\<phi>reason on \<open>\<phi>SemType (?x \<Ztypecolon> \<bool>) ?ty\<close>]:
+  \<open>\<phi>SemType (x \<Ztypecolon> \<bool>) (\<tau>Int 1)\<close>
+  unfolding \<phi>SemType_def subset_iff
+  by (simp add: \<phi>expns)
+
+abbreviation \<open>Predicate_About x \<equiv> (\<bool> <func-over> x)\<close>
+
+
+
+subsection \<open>Variable\<close>
+
+definition Var :: \<open>varname \<Rightarrow> ('VAL,'a) \<phi> \<Rightarrow> 'a \<Rightarrow> ('FIC_N \<Rightarrow> 'FIC) set\<close>
+  where \<open>Var vname T x = {FIC_var.mk (Fine (1(vname \<mapsto> val))) |val. val \<in> (x \<Ztypecolon> T)} \<close>
+
+lemma Var_expn[\<phi>expns]:
+  \<open>fic \<in> (x \<Ztypecolon> Var vname T) \<longleftrightarrow> (\<exists>val. fic = FIC_var.mk (Fine (1(vname \<mapsto> val))) \<and> val \<in> (x \<Ztypecolon> T))\<close>
+  unfolding Var_def \<phi>Type_def by simp
+
+lemma Var_inhabited[\<phi>reason_elim!,elim!]:
+  \<open>Inhabited (x \<Ztypecolon> Var vname T) \<Longrightarrow> (Inhabited (x \<Ztypecolon> T) \<Longrightarrow> C) \<Longrightarrow> C\<close>
+  unfolding Inhabited_def by (simp add: \<phi>expns)
+
+lemma Var_subty:
+  \<open> \<^bold>s\<^bold>u\<^bold>b\<^bold>t\<^bold>y\<^bold>p\<^bold>e x \<Ztypecolon> T \<longmapsto> x' \<Ztypecolon> T' \<^bold>w\<^bold>i\<^bold>t\<^bold>h P
+\<Longrightarrow> \<^bold>s\<^bold>u\<^bold>b\<^bold>t\<^bold>y\<^bold>p\<^bold>e x \<Ztypecolon> Var vname T \<longmapsto> x' \<Ztypecolon> Var vname T' \<^bold>w\<^bold>i\<^bold>t\<^bold>h P\<close>
+  unfolding Subty_def by (simp add: \<phi>expns, blast)
+
+lemma Var_cast_\<phi>app[\<phi>overload cast]: 
+  \<open> \<^bold>a\<^bold>r\<^bold>g\<^bold>u\<^bold>m\<^bold>e\<^bold>n\<^bold>t \<^bold>s\<^bold>u\<^bold>b\<^bold>t\<^bold>y\<^bold>p\<^bold>e x \<Ztypecolon> T \<longmapsto> x' \<Ztypecolon> T' \<^bold>w\<^bold>i\<^bold>t\<^bold>h P
+\<Longrightarrow> \<^bold>s\<^bold>u\<^bold>b\<^bold>t\<^bold>y\<^bold>p\<^bold>e FIX x \<Ztypecolon> Var vname T \<longmapsto> x' \<Ztypecolon> Var vname T' \<^bold>w\<^bold>i\<^bold>t\<^bold>h P\<close>
+  unfolding Argument_def Fix_def
+  using Var_subty .
+
+lemma Var_ExTyp[simp]:
+  \<open>(x \<Ztypecolon> Var vname (ExTyp T)) = (\<exists>*a. x a \<Ztypecolon> Var vname (T a))\<close>
+  unfolding set_eq_iff by (simp add: \<phi>expns, blast)
+
+lemma Var_SubjTyp[simp]:
+  \<open>(x \<Ztypecolon> Var vname (T \<phi>\<^bold>s\<^bold>u\<^bold>b\<^bold>j P)) = (x \<Ztypecolon> Var vname T \<^bold>s\<^bold>u\<^bold>b\<^bold>j P)\<close>
+  unfolding set_eq_iff by (simp add: \<phi>expns, blast)
+
+lemma [\<phi>reason 1200 on \<open>EqualAddress (?xa \<Ztypecolon> Var ?va ?Ta) (?xb \<Ztypecolon> Var ?vb ?Tb)\<close>]:
+  \<open>EqualAddress (xa \<Ztypecolon> Var var Ta) (xb \<Ztypecolon> Var var Tb)\<close>
+  unfolding EqualAddress_def ..
+
+lemma [\<phi>reason 110 on \<open>\<^bold>s\<^bold>u\<^bold>b\<^bold>t\<^bold>y\<^bold>p\<^bold>e ?R \<heavy_comma> ?H \<longmapsto> ?R''' * \<blangle> ?X \<brangle> \<^bold>w\<^bold>i\<^bold>t\<^bold>h ?P \<^bold>@\<^bold>G\<^bold>O\<^bold>A\<^bold>L ?G\<close>]: \<comment> \<open>attempts the immediate cell\<close>
+  " CHK_SUBGOAL G
+\<Longrightarrow> \<^bold>s\<^bold>u\<^bold>b\<^bold>t\<^bold>y\<^bold>p\<^bold>e x \<Ztypecolon> T \<longmapsto> x' \<Ztypecolon> T' \<^bold>w\<^bold>i\<^bold>t\<^bold>h P
+\<Longrightarrow> \<^bold>s\<^bold>u\<^bold>b\<^bold>t\<^bold>y\<^bold>p\<^bold>e R\<heavy_comma> x \<Ztypecolon> Var var T \<longmapsto> R\<heavy_comma> \<blangle> x' \<Ztypecolon> Var var T' \<brangle> \<^bold>w\<^bold>i\<^bold>t\<^bold>h P \<^bold>@\<^bold>G\<^bold>O\<^bold>A\<^bold>L G"
+  unfolding cast_def
+  by (simp add: \<phi>expns times_list_def, blast)
+
+lemma Var_simp_cong:
+  \<open> (x \<Ztypecolon> T) = (x' \<Ztypecolon> T')
+\<Longrightarrow> (x \<Ztypecolon> Var v T) = (x' \<Ztypecolon> Var v T')\<close>
+  unfolding set_eq_iff by (simp add: \<phi>expns)
+
+simproc_setup Var_simp_cong ("x \<Ztypecolon> Var v T") = \<open>
+  K (NuSimpCong.simproc @{thm Var_simp_cong[folded atomize_eq]})
+\<close>
+
+
+subsubsection \<open>Synthesis Rules\<close>
+
+lemma [\<phi>reason on \<open>\<^bold>p\<^bold>r\<^bold>o\<^bold>c ?f \<lbrace> ?S1 \<longmapsto> \<lambda>ret. ?S2\<heavy_comma> SYNTHESIS ?x \<Ztypecolon> Var ?var ?T \<^bold>t\<^bold>h\<^bold>r\<^bold>o\<^bold>w\<^bold>s ?E \<rbrace> \<^bold>@\<^bold>G\<^bold>O\<^bold>A\<^bold>L ?G\<close>]:
+  \<open> SUBGOAL G G'
+\<Longrightarrow> \<^bold>s\<^bold>u\<^bold>b\<^bold>t\<^bold>y\<^bold>p\<^bold>e S1 \<longmapsto> S2\<heavy_comma> \<blangle> x \<Ztypecolon> Var var T \<brangle> \<^bold>@\<^bold>G\<^bold>O\<^bold>A\<^bold>L G'
+\<Longrightarrow> SOLVE_SUBGOAL G'
+\<Longrightarrow> \<^bold>p\<^bold>r\<^bold>o\<^bold>c Success (sem_value ()) \<lbrace> S1 \<longmapsto> S2\<heavy_comma> SYNTHESIS x \<Ztypecolon> Var var T \<rbrace> \<^bold>@\<^bold>G\<^bold>O\<^bold>A\<^bold>L G\<close>
+  unfolding GOAL_CTXT_def FOCUS_TAG_def Synthesis_def
+  using "\<phi>cast" \<phi>reassemble_proc_final
+  by (metis (no_types, lifting) \<phi>SKIP \<phi>apply_proc)
+
+
+subsubsection \<open>Application Methods for Subtyping\<close>
+
+lemma [\<phi>reason 2000 on \<open>
+  PROP \<phi>Application_Method (Trueprop (\<^bold>s\<^bold>u\<^bold>b\<^bold>t\<^bold>y\<^bold>p\<^bold>e ?x \<Ztypecolon> ?T \<longmapsto> ?y \<Ztypecolon> ?U \<^bold>w\<^bold>i\<^bold>t\<^bold>h ?P))
+          (Trueprop (\<^bold>c\<^bold>u\<^bold>r\<^bold>r\<^bold>e\<^bold>n\<^bold>t ?blk [?RR] \<^bold>r\<^bold>e\<^bold>s\<^bold>u\<^bold>l\<^bold>t\<^bold>s \<^bold>i\<^bold>n ?R\<heavy_comma> ?x \<Ztypecolon> Var ?var ?T)) ?Result
+\<close> if no \<open>
+  PROP \<phi>Application_Method (Trueprop (\<^bold>s\<^bold>u\<^bold>b\<^bold>t\<^bold>y\<^bold>p\<^bold>e ?x \<Ztypecolon> Var ?var ?T \<longmapsto> ?y \<Ztypecolon> ?U \<^bold>w\<^bold>i\<^bold>t\<^bold>h ?P))
+          (Trueprop (\<^bold>c\<^bold>u\<^bold>r\<^bold>r\<^bold>e\<^bold>n\<^bold>t ?blk [?RR] \<^bold>r\<^bold>e\<^bold>s\<^bold>u\<^bold>l\<^bold>t\<^bold>s \<^bold>i\<^bold>n ?R)) ?Result
+\<close>]:
+  \<open> PROP \<phi>Application_Success
+\<Longrightarrow> PROP \<phi>Application_Method (Trueprop (\<^bold>s\<^bold>u\<^bold>b\<^bold>t\<^bold>y\<^bold>p\<^bold>e x \<Ztypecolon> T \<longmapsto> y \<Ztypecolon> U \<^bold>w\<^bold>i\<^bold>t\<^bold>h P))
+      (Trueprop (\<^bold>c\<^bold>u\<^bold>r\<^bold>r\<^bold>e\<^bold>n\<^bold>t blk [RR] \<^bold>r\<^bold>e\<^bold>s\<^bold>u\<^bold>l\<^bold>t\<^bold>s \<^bold>i\<^bold>n R\<heavy_comma> x \<Ztypecolon> Var var T))
+      (Trueprop ((\<^bold>c\<^bold>u\<^bold>r\<^bold>r\<^bold>e\<^bold>n\<^bold>t blk [RR] \<^bold>r\<^bold>e\<^bold>s\<^bold>u\<^bold>l\<^bold>t\<^bold>s \<^bold>i\<^bold>n R\<heavy_comma> y \<Ztypecolon> Var var U) \<and> P))\<close>
+  unfolding \<phi>Application_Method_def \<phi>Application_def
+  using "\<phi>cast_P" Var_cast_\<phi>app[unfolded Argument_def Fix_def] \<phi>cast_intro_frame by metis
+
+
+lemma [\<phi>reason 2000 on \<open>
+  PROP \<phi>Application_Method (Trueprop (\<^bold>s\<^bold>u\<^bold>b\<^bold>t\<^bold>y\<^bold>p\<^bold>e ?x' \<Ztypecolon> ?T' \<longmapsto> ?y \<Ztypecolon> ?U \<^bold>w\<^bold>i\<^bold>t\<^bold>h ?P))
+      (Trueprop (\<^bold>c\<^bold>u\<^bold>r\<^bold>r\<^bold>e\<^bold>n\<^bold>t ?blk [?RR] \<^bold>r\<^bold>e\<^bold>s\<^bold>u\<^bold>l\<^bold>t\<^bold>s \<^bold>i\<^bold>n ?R\<heavy_comma> ?x \<Ztypecolon> Var ?var ?T)) ?Result
+\<close> if no \<open>
+  PROP \<phi>Application_Method (Trueprop (\<^bold>s\<^bold>u\<^bold>b\<^bold>t\<^bold>y\<^bold>p\<^bold>e ?x \<Ztypecolon> Var ?var ?T \<longmapsto> ?y \<Ztypecolon> ?U \<^bold>w\<^bold>i\<^bold>t\<^bold>h ?P))
+          (Trueprop (\<^bold>c\<^bold>u\<^bold>r\<^bold>r\<^bold>e\<^bold>n\<^bold>t ?blk [?RR] \<^bold>r\<^bold>e\<^bold>s\<^bold>u\<^bold>l\<^bold>t\<^bold>s \<^bold>i\<^bold>n ?R)) ?Result
+\<close>]:
+  \<open> SUBGOAL TOP_GOAL G
+\<Longrightarrow> \<^bold>s\<^bold>u\<^bold>b\<^bold>t\<^bold>y\<^bold>p\<^bold>e x \<Ztypecolon> T \<longmapsto> x' \<Ztypecolon> T' \<^bold>w\<^bold>i\<^bold>t\<^bold>h Any
+\<Longrightarrow> SOLVE_SUBGOAL G
+\<Longrightarrow> PROP \<phi>Application_Success
+\<Longrightarrow> \<^bold>o\<^bold>b\<^bold>l\<^bold>i\<^bold>g\<^bold>a\<^bold>t\<^bold>i\<^bold>o\<^bold>n True
+\<Longrightarrow> PROP \<phi>Application_Method (Trueprop (\<^bold>s\<^bold>u\<^bold>b\<^bold>t\<^bold>y\<^bold>p\<^bold>e x' \<Ztypecolon> T' \<longmapsto> y \<Ztypecolon> U \<^bold>w\<^bold>i\<^bold>t\<^bold>h P))
+      (Trueprop (\<^bold>c\<^bold>u\<^bold>r\<^bold>r\<^bold>e\<^bold>n\<^bold>t blk [RR] \<^bold>r\<^bold>e\<^bold>s\<^bold>u\<^bold>l\<^bold>t\<^bold>s \<^bold>i\<^bold>n R\<heavy_comma> x \<Ztypecolon> Var var T))
+      (Trueprop ((\<^bold>c\<^bold>u\<^bold>r\<^bold>r\<^bold>e\<^bold>n\<^bold>t blk [RR] \<^bold>r\<^bold>e\<^bold>s\<^bold>u\<^bold>l\<^bold>t\<^bold>s \<^bold>i\<^bold>n R\<heavy_comma> y \<Ztypecolon> Var var U) \<and> P))\<close>
+  unfolding \<phi>Application_Method_def \<phi>Application_def
+  using "\<phi>cast_P" Var_cast_\<phi>app[unfolded Argument_def Fix_def] \<phi>cast_intro_frame by metis
+
+
+subsubsection \<open>Branch Convergence Rules\<close>
+
+lemma [\<phi>reason 1200 on
+  \<open>\<^bold>c\<^bold>o\<^bold>n\<^bold>v[branch_convergence] Merge ?P (?R1 \<heavy_comma> ?x \<Ztypecolon> Var ?v ?T) (?N \<heavy_comma> \<blangle> ?R2 \<heavy_comma> ?y \<Ztypecolon> Var ?v' ?U \<brangle>) = ?X \<^bold>@\<^bold>G\<^bold>O\<^bold>A\<^bold>L ?G\<close>
+]:
+  " \<^bold>c\<^bold>o\<^bold>n\<^bold>v[branch_convergence] Merge P (x \<Ztypecolon> T) (y \<Ztypecolon> U) = (z \<Ztypecolon> Z)
+\<Longrightarrow> \<^bold>c\<^bold>o\<^bold>n\<^bold>v[branch_convergence] Merge P R1 (1 \<heavy_comma> \<blangle> N \<heavy_comma> R2 \<brangle>) = R \<^bold>@\<^bold>G\<^bold>O\<^bold>A\<^bold>L G
+\<Longrightarrow> \<^bold>c\<^bold>o\<^bold>n\<^bold>v[branch_convergence] Merge P (R1 \<heavy_comma> x \<Ztypecolon> Var v T) (N \<heavy_comma> \<blangle> R2 \<heavy_comma> y \<Ztypecolon> Var v U \<brangle>) = (R \<heavy_comma> z \<Ztypecolon> Var v Z) \<^bold>@\<^bold>G\<^bold>O\<^bold>A\<^bold>L G"
+  unfolding Conv_def cast_def Merge_def by (cases P; simp add: \<phi>expns mult.assoc)
+
+declare branch_convergence_skip[\<phi>reason 1200
+     on \<open>\<^bold>c\<^bold>o\<^bold>n\<^bold>v[branch_convergence] Merge ?P (?R1 \<heavy_comma> ?x \<Ztypecolon> Var ?v ?T) (?N \<heavy_comma> \<blangle> ?R2 \<heavy_comma> ?Y \<brangle>) = ?R \<^bold>@\<^bold>G\<^bold>O\<^bold>A\<^bold>L ?G\<close>
+  if no \<open>\<^bold>c\<^bold>o\<^bold>n\<^bold>v[branch_convergence] Merge ?P (?R1 \<heavy_comma> ?x \<Ztypecolon> Var ?v ?T) (?N \<heavy_comma> \<blangle> ?R2 \<heavy_comma> ?y \<Ztypecolon> Var ?v' ?U \<brangle>) = ?R \<^bold>@\<^bold>G\<^bold>O\<^bold>A\<^bold>L ?rG\<close>
+]
+
+end
+
+
+section \<open>Instructions\<close>
+
+context \<phi>min_sem begin
+
+subsection \<open>Arithmetic Operations\<close>
+
+subsubsection \<open>Integer arithmetic\<close>
+
+definition op_const_int :: "nat \<Rightarrow> nat \<Rightarrow> ('VAL,'RES_N,'RES) proc"
+  where "op_const_int bits const = Success (sem_value (V_int.mk (bits,const)))"
+
+definition op_const_size_t :: "nat \<Rightarrow> ('VAL,'RES_N,'RES) proc"
+  where "op_const_size_t c = \<phi>M_assume (c < 2 ^ addrspace_bits)
+                          \<ggreater> Success (sem_value (V_int.mk (addrspace_bits,c)))"
+  \<comment> \<open> `op_const_size_t` checks the overflow during the compilation towards certain decided platform.  \<close>
+
+definition op_add :: "nat \<Rightarrow> ('VAL \<times> 'VAL, 'VAL, 'RES_N, 'RES) proc'"
+  where "op_add bits =
+      \<phi>M_caseV (\<lambda>va vb.
+      \<phi>M_getV (\<tau>Int bits) (snd o V_int.dest) va (\<lambda>val_a.
+      \<phi>M_getV (\<tau>Int bits) (snd o V_int.dest) vb (\<lambda>val_b.
+      Success (sem_value (V_int.mk (bits, ((val_a + val_b) mod 2^bits))))
+  )))"
+
+
+(* lemma (in \<phi>empty) op_add:
+  \<open> \<^bold>p\<^bold>r\<^bold>e\<^bold>m\<^bold>i\<^bold>s\<^bold>e x + y < 2^b
+\<Longrightarrow> \<^bold>p\<^bold>r\<^bold>o\<^bold>c op_add b (\<phi>V_pair vb va) \<lbrace> x \<Ztypecolon> Val va \<nat>[b]\<heavy_comma> y \<Ztypecolon> Val vb \<nat>[b] \<longmapsto> \<^bold>v\<^bold>a\<^bold>l x + y \<Ztypecolon> \<nat>[b] \<rbrace>\<close>
+  unfolding op_add_def Premise_def
+  by (cases va; cases vb; simp, \<phi>reason) *)
+
+
+(* lemma (in \<phi>empty)
+  \<open> \<^bold>p\<^bold>r\<^bold>o\<^bold>c left  \<lbrace> R1 \<longmapsto> R2\<heavy_comma> SYNTHESIS x \<Ztypecolon> \<nat>[b] \<rbrace>
+\<Longrightarrow> \<^bold>p\<^bold>r\<^bold>o\<^bold>c right \<lbrace> R2 \<longmapsto> R3\<heavy_comma> SYNTHESIS y \<Ztypecolon> \<nat>[b] \<rbrace>
+\<Longrightarrow> \<^bold>p\<^bold>r\<^bold>e\<^bold>m\<^bold>i\<^bold>s\<^bold>e x + y < 2^b
+\<Longrightarrow> \<^bold>p\<^bold>r\<^bold>o\<^bold>c (left \<ggreater> right \<ggreater> op_add b) \<lbrace> R1 \<longmapsto> R3\<heavy_comma> SYNTHESIS x + y \<Ztypecolon> \<nat>[b] \<rbrace>\<close>
+  apply (\<phi>reason, assumption) *)
+
+definition op_sub :: "nat \<Rightarrow> ('VAL \<times> 'VAL, 'VAL, 'RES_N, 'RES) proc'"
+  where "op_sub bits =
+      \<phi>M_caseV (\<lambda>va vb.
+      \<phi>M_getV (\<tau>Int bits) (snd o V_int.dest) va (\<lambda>val_a.
+      \<phi>M_getV (\<tau>Int bits) (snd o V_int.dest) vb (\<lambda>val_b.
+      Success (sem_value (V_int.mk (bits, ((2^bits + val_b - val_a) mod 2^bits))))
+  )))"
+
+definition op_umul :: "nat \<Rightarrow> ('VAL \<times> 'VAL, 'VAL, 'RES_N, 'RES) proc'"
+  where "op_umul bits =
+      \<phi>M_caseV (\<lambda>va vb.
+      \<phi>M_getV (\<tau>Int bits) (snd o V_int.dest) va (\<lambda>val_a.
+      \<phi>M_getV (\<tau>Int bits) (snd o V_int.dest) vb (\<lambda>val_b.
+      Success (sem_value (V_int.mk (bits, ((val_b * val_a) mod 2^bits))))
+  )))"
+
+definition op_udiv :: "nat \<Rightarrow> ('VAL \<times> 'VAL, 'VAL, 'RES_N, 'RES) proc'"
+  where "op_udiv bits =
+      \<phi>M_caseV (\<lambda>va vb.
+      \<phi>M_getV (\<tau>Int bits) (snd o V_int.dest) va (\<lambda>val_a.
+      \<phi>M_getV (\<tau>Int bits) (snd o V_int.dest) vb (\<lambda>val_b.
+      Success (sem_value (V_int.mk (bits, (val_b div val_a))))
+  )))"
+
+definition op_lt :: "nat \<Rightarrow> ('VAL \<times> 'VAL, 'VAL,'RES_N,'RES) proc'"
+  where "op_lt bits =
+      \<phi>M_caseV (\<lambda>va vb.
+      \<phi>M_getV (\<tau>Int bits) (snd o V_int.dest) va (\<lambda>val_a.
+      \<phi>M_getV (\<tau>Int bits) (snd o V_int.dest) vb (\<lambda>val_b.
+      Success (sem_value (V_int.mk (1, (if val_b < val_a then 1 else 0))))
+  )))"
+
+
+definition op_le :: "nat \<Rightarrow> ('VAL \<times> 'VAL, 'VAL,'RES_N,'RES) proc'"
+  where "op_le bits =
+      \<phi>M_caseV (\<lambda>va vb.
+      \<phi>M_getV (\<tau>Int bits) (snd o V_int.dest) va (\<lambda>val_a.
+      \<phi>M_getV (\<tau>Int bits) (snd o V_int.dest) vb (\<lambda>val_b.
+      Success (sem_value (V_int.mk (1, (if val_b \<le> val_a then 1 else 0))))
+  )))"
+
+
+definition op_not :: "('VAL, 'VAL,'RES_N,'RES) proc'"
+  where "op_not v =
+    \<phi>M_getV (\<tau>Int 1) (snd o V_int.dest) v (\<lambda>v.
+    Success (sem_value (V_int.mk (1, 1 - v)))
+  )"
+
+definition op_and :: "('VAL \<times> 'VAL, 'VAL,'RES_N,'RES) proc'"
+  where "op_and =
+    \<phi>M_caseV (\<lambda>va vb.
+    \<phi>M_getV (\<tau>Int 1) (snd o V_int.dest) va (\<lambda>v.
+    \<phi>M_getV (\<tau>Int 1) (snd o V_int.dest) vb (\<lambda>u.
+    Success (sem_value (V_int.mk (1, v+u-1)))
+  )))"
+
+definition op_or :: "('VAL \<times> 'VAL, 'VAL,'RES_N,'RES) proc'"
+  where "op_or =
+    \<phi>M_caseV (\<lambda>va vb.
+    \<phi>M_getV (\<tau>Int 1) (snd o V_int.dest) va (\<lambda>v.
+    \<phi>M_getV (\<tau>Int 1) (snd o V_int.dest) vb (\<lambda>u.
+    Success (sem_value (V_int.mk (1, min 1 (v+u))))
+  )))"
+
+definition op_equal :: "'TY \<Rightarrow> ('VAL \<times> 'VAL, 'VAL,'RES_N,'RES) proc'"
+  where "op_equal TY =
+    \<phi>M_caseV (\<lambda>va vb.
+    \<phi>M_getV TY id va (\<lambda>v.
+    \<phi>M_getV TY id vb (\<lambda>u.
+    (\<lambda>res. \<phi>M_assert (Can_EqCompare res u v) res) \<ggreater>
+    Success (sem_value (V_int.mk (1, (if EqCompare u v then 1 else 0))))
+)))"
+
+
+
+
+subsection \<open>Variable Operations\<close>
+
+definition \<phi>M_get_var
+    :: "varname \<Rightarrow> 'TY \<Rightarrow> ('VAL \<Rightarrow> ('ret,'RES_N,'RES) proc) \<Rightarrow> ('ret,'RES_N,'RES) proc"
+  where "\<phi>M_get_var vname TY F = R_var.\<phi>R_get_res_entry vname (\<lambda>val.
+            \<phi>M_assert (val \<in> Well_Type TY) \<ggreater> F val)"
+
+definition op_get_var :: "varname \<Rightarrow> 'TY \<Rightarrow> ('VAL,'RES_N,'RES) proc"
+  where "op_get_var vname TY = \<phi>M_get_var vname TY (\<lambda>x. Success (sem_value x))"
+
+definition op_set_var :: "varname \<Rightarrow> 'TY \<Rightarrow> ('VAL, unit, 'RES_N, 'RES) proc'"
+  where "op_set_var vname TY v =
+          \<phi>M_getV TY id v (\<lambda>v.
+          \<phi>M_get_var vname TY (\<lambda>_.
+          R_var.\<phi>R_set_res (\<lambda>f. f(vname := Some v))))"
+
+definition op_free_var :: "varname \<Rightarrow> (unit,'RES_N,'RES) proc"
+  where "op_free_var vname = R_var.\<phi>R_set_res (\<lambda>f. f(vname := None))"
+
+definition op_var_scope' :: "'TY
+                          \<Rightarrow> (varname \<Rightarrow> ('ret,'RES_N,'RES) proc)
+                          \<Rightarrow> ('VAL,'ret,'RES_N,'RES) proc'"
+  where "op_var_scope' TY F v =
+    \<phi>M_getV TY id v (\<lambda>v.
+    R_var.\<phi>R_allocate_res_entry (\<lambda>_. True) (Some v) F
+  )"
+
+lemma (in \<phi>min) \<phi>M_get_var[\<phi>reason!]:
+  \<open> v \<in> Well_Type TY
+\<Longrightarrow> \<^bold>p\<^bold>r\<^bold>o\<^bold>c F v \<lbrace> v \<Ztypecolon> Var vname Identity \<longmapsto> Y \<rbrace>
+\<Longrightarrow> \<^bold>p\<^bold>r\<^bold>o\<^bold>c \<phi>M_get_var vname TY F \<lbrace> v \<Ztypecolon> Var vname Identity \<longmapsto> Y \<rbrace>\<close>
+  unfolding \<phi>Procedure_\<phi>Res_Spec \<phi>M_get_var_def
+  by (clarsimp simp add: \<phi>expns FIC_var.expand, rule R_var.\<phi>R_get_res_entry[where v=v]; simp)
+
+lemma (in \<phi>min) \<phi>M_set_var[\<phi>reason!]:
+  \<open>\<^bold>p\<^bold>r\<^bold>o\<^bold>c R_var.\<phi>R_set_res (\<lambda>f. f(vname \<mapsto> u)) \<lbrace> v \<Ztypecolon> Var vname Identity \<longmapsto> \<lambda>_. u \<Ztypecolon> Var vname Identity \<rbrace>\<close>
+  unfolding \<phi>Procedure_\<phi>Res_Spec
+  by (clarsimp simp add: \<phi>expns FIC_var.expand, rule R_var.\<phi>R_set_res[where P=\<open>\<lambda>_. True\<close>]; simp)
+
+lemma (in \<phi>min) op_get_var''_\<phi>app:
+   \<open>\<^bold>p\<^bold>r\<^bold>e\<^bold>m\<^bold>i\<^bold>s\<^bold>e v \<in> Well_Type TY
+    \<Longrightarrow> \<^bold>p\<^bold>r\<^bold>o\<^bold>c op_get_var vname TY \<lbrace> v \<Ztypecolon> Var vname Identity \<longmapsto> v \<Ztypecolon> Var vname Identity \<heavy_comma> \<^bold>v\<^bold>a\<^bold>l v \<Ztypecolon> Identity \<rbrace>\<close>
+  unfolding op_get_var_def Premise_def
+  by (\<phi>reason, assumption, \<phi>reason)
+
+end
+
+
+lemma (in \<phi>min) op_set_var''_\<phi>app:
+   \<open>\<^bold>p\<^bold>r\<^bold>e\<^bold>m\<^bold>i\<^bold>s\<^bold>e v \<in> Well_Type TY
+\<Longrightarrow> \<^bold>p\<^bold>r\<^bold>e\<^bold>m\<^bold>i\<^bold>s\<^bold>e u \<in> Well_Type TY
+\<Longrightarrow> \<^bold>p\<^bold>r\<^bold>o\<^bold>c op_set_var vname TY rawv \<lbrace> v \<Ztypecolon> Var vname Identity\<heavy_comma> u \<Ztypecolon> Val rawv Identity \<longmapsto> u \<Ztypecolon> Var vname Identity \<rbrace>\<close>
+  unfolding op_set_var_def Premise_def
+  by (cases rawv; simp, \<phi>reason, assumption, simp add: \<phi>expns, \<phi>reason)
+
+lemma (in \<phi>min) op_var_scope':
+   \<open>\<^bold>p\<^bold>r\<^bold>e\<^bold>m\<^bold>i\<^bold>s\<^bold>e v \<in> Well_Type TY
+\<Longrightarrow> (\<And>vname. \<^bold>p\<^bold>r\<^bold>o\<^bold>c F vname \<lbrace> X\<heavy_comma> v \<Ztypecolon> Var vname Identity \<longmapsto> Y \<^bold>t\<^bold>h\<^bold>r\<^bold>o\<^bold>w\<^bold>s E \<rbrace> )
+\<Longrightarrow> \<^bold>p\<^bold>r\<^bold>o\<^bold>c op_var_scope' TY F rawv \<lbrace> X\<heavy_comma> v \<Ztypecolon> Val rawv Identity \<longmapsto> Y \<^bold>t\<^bold>h\<^bold>r\<^bold>o\<^bold>w\<^bold>s E \<rbrace>\<close>
+  unfolding op_var_scope'_def Premise_def
+  apply (cases rawv; simp, \<phi>reason)
+  apply (clarsimp simp add: \<phi>expns \<phi>Procedure_\<phi>Res_Spec)
+  subgoal for r res c
+  apply (rule R_var.\<phi>R_allocate_res_entry[where R="(\<I> INTERP (r * c))"])
+     apply (clarsimp) using finite_map_freshness infinite_varname apply blast
+      apply (clarsimp)
+  apply (clarsimp simp add: FIC_var.expand[symmetric] mult.assoc)
+  subgoal premises prems for k res'
+    apply (rule prems(2)[THEN spec[where x=r], THEN spec[where x=res'],
+                simplified prems, simplified, THEN mp])
+    using Fic_Space_mm prems(5) prems(7) prems(8) by blast . .
+
+
+lemma (in \<phi>min) op_free_var:
+   \<open>\<^bold>p\<^bold>r\<^bold>o\<^bold>c op_free_var vname \<lbrace> v \<Ztypecolon> Var vname Identity \<longmapsto> 1 \<rbrace>\<close>
+  unfolding op_free_var_def \<phi>Procedure_\<phi>Res_Spec
+  apply (clarsimp simp add: \<phi>expns FIC_var.expand)
+  apply (rule R_var.\<phi>R_dispose_res[where any=v])
+  apply clarsimp .
+
+
+subsection \<open>Branches & Loops\<close>
+
+context \<phi>min_sem begin
+
+paragraph \<open>Non-Branching Selection\<close>
+
+definition op_sel :: "'TY \<Rightarrow> ('VAL \<times> 'VAL \<times> 'VAL, 'VAL,'RES_N,'RES) proc'"
+  where "op_sel TY =
+    \<phi>M_caseV (\<lambda>vc. \<phi>M_caseV (\<lambda>va vb.
+    \<phi>M_getV (\<tau>Int 1) V_int.dest vc (\<lambda>c.
+    \<phi>M_getV TY id va (\<lambda>a.
+    \<phi>M_getV TY id vb (\<lambda>b.
+    Success (sem_value (if snd c = 1 then b else a)))))))"
+
+paragraph \<open>Branch\<close>
+
+definition op_if :: "('ret,'RES_N,'RES) proc
+                  \<Rightarrow> ('ret,'RES_N,'RES) proc
+                  \<Rightarrow> ('VAL,'ret,'RES_N,'RES) proc'"
+  where "op_if brT brF v =
+    \<phi>M_getV (\<tau>Int 1) V_int.dest v (\<lambda>c. (if snd c = 1 then brT else brF))"
+
+paragraph \<open>While Loop\<close>
+
+inductive SemDoWhile :: "('VAL,'RES_N,'RES) proc \<Rightarrow> ('RES_N \<Rightarrow> 'RES) \<Rightarrow> (unit,'RES_N,'RES) state \<Rightarrow> bool" where
+  "f s = Success (sem_value (V_int.mk (1,0))) res \<Longrightarrow> SemDoWhile f s (Success (sem_value ()) res)"
+| "f s = Success (sem_value (V_int.mk (1,1))) res \<Longrightarrow> SemDoWhile f res s'' \<Longrightarrow> SemDoWhile f s s''"
+| "f s = Exception e \<Longrightarrow> SemDoWhile f s (Exception e)"
+| "f s = PartialCorrect \<Longrightarrow> SemDoWhile f s PartialCorrect"
+| "f s = Fail \<Longrightarrow> SemDoWhile f s Fail"
+
+lemma "\<nexists> y. SemDoWhile (\<lambda>res. Success (sem_value (V_int.mk (1,1))) res) res y"
+  apply rule apply (elim exE) subgoal for y 
+    thm SemDoWhile.induct
+    apply (induct "(\<lambda>res. Success (sem_value (V_int.mk (1,1))) (res::'RES_N \<Rightarrow> 'RES))" res y
+           rule: SemDoWhile.induct)
+       apply simp_all
+    done done
+
+definition op_do_while :: "('VAL,'RES_N,'RES) proc \<Rightarrow> (unit,'RES_N,'RES) proc" where
+  "op_do_while f s = (if (\<exists>y. SemDoWhile f s y) then The (SemDoWhile f s) else PartialCorrect)"
+
+lemma SemDoWhile_deterministic:
+  assumes "SemDoWhile c s s1"
+      and "SemDoWhile c s s2"
+    shows "s1 = s2"
+proof -
+  have "SemDoWhile c s s1 \<Longrightarrow> (\<forall>s2. SemDoWhile c s s2 \<longrightarrow> s1 = s2)"
+    apply (induct rule: SemDoWhile.induct)
+    by (subst SemDoWhile.simps, simp)+
+  thus ?thesis
+    using assms by simp
+qed
+
+lemma SemDoWhile_deterministic2:
+    "SemDoWhile body s x \<Longrightarrow> The ( SemDoWhile body s) = x"
+  using SemDoWhile_deterministic by blast
+
+
+paragraph \<open>Recursion\<close>
+
+inductive SemRec :: "(('a,'a,'RES_N,'RES) proc' \<Rightarrow> ('a,'a,'RES_N,'RES) proc')
+            \<Rightarrow> 'a sem_value \<Rightarrow> ('RES_N \<Rightarrow> 'RES) \<Rightarrow> ('a,'RES_N,'RES) state \<Rightarrow> bool"
+where
+  SemRec_I0: "(\<And>g. F g x res = y) \<Longrightarrow> SemRec F x res y"
+| SemRec_IS: "SemRec (F o F) x res y \<Longrightarrow> SemRec F x res y"
+
+definition op_recursion :: "'TY list \<Rightarrow> 'TY list
+                         \<Rightarrow> (('a,'a,'RES_N,'RES) proc' \<Rightarrow> ('a,'a,'RES_N,'RES) proc')
+                         \<Rightarrow> ('a,'a,'RES_N,'RES) proc'"
+  where "op_recursion _ _ F x s = (if (\<exists>t. SemRec F x s t) then The (SemRec F x s) else PartialCorrect)"
+
+
+end
+
+end
+
+
